\documentclass[a4paper, 12pt]{article}

\usepackage{mathexam}
\usepackage{amsmath}
\usepackage{amsfonts}
\usepackage{graphicx}
\usepackage{systeme}
\usepackage{microtype}
\usepackage{multirow}
\usepackage{pgfplots}
\usepackage{listings}
\usepackage{tikz}
\usepackage{dsfont} %Numeros reales, naturales...
\usepackage{verbatimbox} %comentarios

%\graphicspath{{images/}}
\newcommand*{\qed}{\hfill\ensuremath{\square}}

%Estructura de ecuaciones
\setlength{\textwidth}{15cm} \setlength{\oddsidemargin}{5mm}
\setlength{\textheight}{23cm} \setlength{\topmargin}{-1cm}



\author{David Garc√≠a Curbelo}
\title{Probabilidad}
\date{Marginales y Condicionadas del ejercicio 1 tema 2 parte II}

\pagestyle{empty}



\def\R{\mathds{R}}
\def\sup{$^2$}

\begin{document}
    \maketitle
    \setcounter{page}{1}
    \pagestyle{plain}

    {\bf{Marginales}}\\ \\
    $$f_X(x)=\int_{-\frac{2}{3}(x+3)}^{\frac{2}{3}x+ 2}k dy=
    \left(\frac{4}{3}x+4\right), \quad \forall x \in [-3,0]$$\\ \\
    
    $$f_X(x)=\int_{\frac{2}{3}x-2}^{2-\frac{2}{3}x}k dy=
    k\left(5-\frac{4}{3}x\right), \quad \forall x \in [0,3]$$\\ \\

    $$f_Y(y)=\int_{\frac{3}{2}(y-2)}^{\frac{3}{2}(3-y)}k dx =
    k\left(\frac{3}{2}(3-y)-\frac{3}{2}(y-2)\right), \quad \forall y \in [0,2] $$\\ \\

    $$f_Y(y)=\int_{\frac{3}{2}(3-y)}^{\frac{3}{2}(y+2)}k dx =
    k\left(\frac{3}{2}(y+2)-\frac{3}{2}(3-y)\right), \quad \forall y \in [0,2] $$\\ \\

    \newpage

    {\bf{Condicionadas}}\\ \\

        $$f_{X/Y=y_0}(x)=\frac{f_{(X,Y)}(x,y_0)}{f_Y(y_0)}=\frac{1}{(3-y_0)3/2 - (y_0-2)3/2}$$
        $$\quad y_0 \in [0,2], \quad \forall x \in \left[(y_0-2)3/2, (3-y_0)3/2\right]$$\\ \\

        $$f_{X/Y=y_0}(x)=\frac{f_{(X,Y)}(x,y_0)}{f_Y(y_0)}=\frac{1}{(2+y_0)3/2 - (3-y_0)3/2}$$
        $$\quad y_0 \in [-2,0], \quad \forall x \in \left[((3-y_0)3/2, (2+y_0)3/2\right]$$\\ \\

        $$f_{Y/X=x_0}(y)=\frac{f_{(X,Y)}(x_0,y)}{f_X(x_0)}=\frac{1}{(3+x_0)2/3 + (3+x_0)2/3}$$
        $$\quad x_0 \in [-3,0], \quad \forall y \in \left[(-(3+x_0)2/3, (3+x_0)2/3\right]$$\\ \\

        $$f_{Y/X=x_0}(y)=\frac{f_{(X,Y)}(x_0,y)}{f_X(x_0)}=\frac{1}{3-2/3x_0 + (3-x_0)2/3}$$
        $$\quad x_0 \in [0,3], \quad \forall y \in \left[(\frac{2}{3}x_0-2, 2-\frac{2}{3}x_0\right]$$\\ \\


\end{document}